feat: preservation defination

CollapsingTowers/TwoLevelPCP/Preservation.lean
@@ -1,2 +1,54 @@
 
 import CollapsingTowers.TwoLevelPCP.Typing
+import CollapsingTowers.TwoLevelPCP.Shift
+@[simp]
+def dyn_env (Γ : TEnv) : Prop :=
+  ∀ x τ 𝕊, binds x τ 𝕊 Γ -> 𝕊 = .dyn
+
+theorem preservation_subst_strengthened :
+    ∀ Γ Δ Φ v e τ𝕒 τ𝕓 φ,
+      typing Γ .stat e τ𝕓 φ ->
+      Γ = Δ ++ (τ𝕒, .stat) :: Φ ->
+      typing Φ .stat v τ𝕒 ∅ ->
+      typing (Δ ++ Φ) .stat (shiftr_at Φ.length (subst Φ.length v e)) τ𝕓 φ :=
+  by
+  intros Γ Δ Φ v e τ𝕒 τ𝕓 φ Hτe HEqΓ Hτv
+  admit
+
+theorem preservation_head𝕄 :
+    ∀ Γ e₀ e₁ τ φ,
+      dyn_env Γ ->
+      head𝕄 e₀ e₁ ->
+      lc e₀ ->
+      typing Γ .stat e₀ τ φ ->
+      typing Γ .stat e₁ τ φ :=
+  by
+  intros Γ e₀ e₁ τ φ HdynΓ Hhead Hlc Hτ
+  cases Hhead
+  case lets Hvalue => admit
+  all_goals admit
+
+theorem preservation_strengthened :
+    ∀ Γ e₀ e₁ τ φ₀,
+      dyn_env Γ ->
+      step_lvl Γ.length e₀ e₁ ->
+      typing_reification Γ e₀ τ φ₀ ->
+      ∃ φ₁, typing_reification Γ e₁ τ φ₁ ∧ φ₁ <= φ₀ :=
+  by
+  intro Γ e₀ e₁ τ φ₀
+  generalize HEqlvl : Γ.length = lvl
+  intro HdynΓ Hstep Hτ; cases Hstep
+  case step𝕄 HM Hlc Hhead𝕄 =>
+    induction HM generalizing τ Γ
+    case hole =>
+      exists φ₀; constructor
+      . cases Hτ
+        all_goals
+          (next Hτ =>
+              constructor
+              apply preservation_head𝕄
+              apply HdynΓ; apply Hhead𝕄; apply Hlc; apply Hτ)
+      . rfl
+    case cons𝔹 HB _ IHM => admit
+    case consℝ HR HM IHM => admit
+  case reflect => admit
