CollapsingTowers/TwoLevelPCP/Effect.lean
@@ -1,4 +1,5 @@
 
+import Mathlib.Order.Basic
 inductive Effects : Type where
   | pure
   | reflect
@@ -10,10 +11,30 @@ def union : Effects → Effects → Effects
   | _, .reflect => .reflect
 
 @[simp]
+def le : Effects → Effects → Prop
+  | .pure, _ => true
+  | .reflect, .reflect => true
+  | _, _ => false
+
+@[simp]
 instance : EmptyCollection Effects where emptyCollection := .pure
 
 @[simp]
 instance : Union Effects where union := union
+
+@[simp]
+instance : LE Effects where le := le
+
+instance : Preorder Effects where
+  le_refl := by intro x; cases x <;> simp
+  le_trans := by intros x y z; cases x <;> cases y <;> cases z <;> simp
+  lt_iff_le_not_le := by intros x y; cases x <;> cases y <;> simp
+
+instance : PartialOrder Effects where
+  le_antisymm := by
+    intros x y
+    cases x <;> cases y <;> simp
+    all_goals intro _ _; contradiction
 
 theorem union_empty : forall φ : Effects, φ ∪ ∅ = φ := by
   intro φ
